src/ModularArithmetic/PseudoMersenneBaseParams.v
@@ -15,6 +15,7 @@ Class PseudoMersenneBaseParams (modulus : Z) := {
   prime_modulus : Znumtheory.prime modulus;
   k := sum_firstn limb_widths (length limb_widths);
   c := 2 ^ k - modulus;
+  c_pos : 0 < c;
   limb_widths_match_modulus : forall i j,
     (i < length limb_widths)%nat ->
     (j < length limb_widths)%nat ->
